pcuic/theories/PCUICParallelReduction.v
@@ -80,7 +80,7 @@ Lemma term_forall_ctx_list_ind :
     (forall Γ (n : name) (t : term),
         P Γ t -> forall t0 : term, P Γ t0 -> forall t1 : term, P (vdef n t t0 :: Γ) t1 -> P Γ (tLetIn n t t0 t1)) ->
     (forall Γ (t u : term), P Γ t -> P Γ u -> P Γ (tApp t u)) ->
-    (forall Γ (s : String.string) (u : list Level.t), P Γ (tConst s u)) ->
+    (forall Γ s (u : list Level.t), P Γ (tConst s u)) ->
     (forall Γ (i : inductive) (u : list Level.t), P Γ (tInd i u)) ->
     (forall Γ (i : inductive) (n : nat) (u : list Level.t), P Γ (tConstruct i n u)) ->
     (forall Γ (p : inductive * nat) (t : term),
@@ -807,13 +807,13 @@ Section ParallelReduction.
           unfold_cofix mfix1 idx = Some (narg, fn) ->
           All2 (P' Γ Γ') args0 args1 ->
           P Γ Γ' (tProj p (mkApps (tCoFix mfix0 idx) args0)) (tProj p (mkApps fn args1))) ->
-      (forall (Γ Γ' : context) (c : ident) (decl : constant_body) (body : term),
+      (forall (Γ Γ' : context) c (decl : constant_body) (body : term),
           All2_local_env (on_decl pred1) Γ Γ' ->
           Pctx Γ Γ' ->
           declared_constant Σ c decl ->
           forall u : Instance.t, cst_body decl = Some body ->
                                         P Γ Γ' (tConst c u) (subst_instance_constr u body)) ->
-      (forall (Γ Γ' : context) (c : ident) (u : Instance.t),
+      (forall (Γ Γ' : context) c (u : Instance.t),
           All2_local_env (on_decl pred1) Γ Γ' ->
           Pctx Γ Γ' ->
           P Γ Γ' (tConst c u) (tConst c u)) ->
@@ -1839,9 +1839,8 @@ Section ParallelSubstitution.
 
     - autorewrite with subst. simpl.
       unfold unfold_cofix in heq_unfold_cofix.
-      destruct (nth_error mfix1 idx) eqn:Hnth; noconf heq_unfold_cofix. simpl.
-      econstructor; pcuic.
-      eapply X0; pcuic.
+      destruct (nth_error mfix1 idx) eqn:Hnth; noconf heq_unfold_cofix.
+      econstructor; eauto.
       rewrite !subst_fix_context.
       erewrite subst_fix_context.
       eapply All2_local_env_subst_ctx; pcuic.
