translations/param_generous_packed.v
@@ -16,8 +16,11 @@ Definition pair (typ1 typ2 t1 t2 : term) : term
   := tApp tPair [ typ1 ; typ2 ; t1 ; t2].
 Definition pack (t u : term) : term
   := tApp tSigma [ t ; u ].
-Definition sigma_ind := Eval compute in
-  match tSigma with tInd i _ => i | _ =>  mkInd "bug: sigma not an inductive" 0 end.
+MetaCoq Run (t <- tmQuote (@sigT) ;;
+            match t with
+            | tInd i _ => tmDefinition "sigma_ind" i
+            | _ => tmFail "bug"
+            end).
 Definition proj1 (t : term) : term
   := tProj (sigma_ind, 2, 0) t.
 Definition proj2 (t : term) : term
